$$ S = \sum\limits_{i=1}^n a_i $$

$$ p_{i,j} = P(a_i = j) $$

$$ S^2 = \sum\limits_{i=1}^n \sum\limits_{j=1}^n a_i \times a_j $$

$$ S_i \subset \{ 1, 2, 3, ... n \} $$

$$ b_i = \prod\limits_{j \in S_i} a_j $$

$$ E((\sum b_i)^2) = \sum \sum E( b_i \times b_j ) = \sum\limits_{i=1}^n \sum\limits_{j=1}^n [i = j] = n $$

$$ S_i \oplus S_j = \empty \to b_i = b_j \to E(b_i \times b_j) = 1 $$

$$ S_i \oplus S_j \ne \empty, E(b_i \times b_j) = 1 \times 1/2 + -1 \times 1/2 = 0 $$

$$ \sum \sum \sum \sum E(b_i \times b_j \times b_k \times b_l) $$

$$ S \oplus T = \{ i, i \in S, i \notin T æˆ– i \in T, i \notin S \} $$

$$ \{ 1,2,3 \} \oplus \{ 1,3,4 \} = \{ 2,4 \} $$

$$ (a_1 \times a_2 \times a_3) \times (a_1 \times a_3 \times a_4) = a_2 \times a_4 $$

$$ S_i \oplus S_j = S_k $$

$$ b_i \times b_j = b_k $$

$$ S_i \oplus S_j \oplus S_k \oplus S_l = \empty \to E(...) = 1 $$

$$ ... \ne \empty \to E(...) = 0 $$

$$ \sum \sum \sum \sum [ S_i \oplus S_j \oplus S_k \oplus S_l = \empty ] $$
$$ E(X^2) = \sum\limits_{i=1}^{n}\sum\limits_{j=1}^{n+1}(j-i)^2 \frac{1}{\binom{2}{n-1}}$$

$$ E(X)=0=50\% \times -1 +50\% \times 1=0  $$

$$ E(X^2) = \sum\limits_{i=1}^{n}\sum\limits_{j=1}^{n+1}(j-i)^2 \frac{1}{\binom{2}{n-1}}$$
$$ E(X^2)=\frac{n(n+1)}{\binom{2}{n+1}}
 $$

 $$ E(X^4)=E(E(X^2))=E(\frac{n(n+1)}{\binom{2}{n+1}}^2) $$

 $$  $$