$$ \binom{n}{m} \equiv \binom{n/p}{m/p} \times \binom{n \bmod p}{m \bmod p} \pmod{p} $$

$$ \binom{p}{n} \equiv [n = 0 或 n = p] \pmod{p} $$

$$ \binom{p}{n} = \frac{p!}{n! (p-n)!} $$

$$ (1+x)^p = \sum\limits_{i=0}^p \binom{p}{i} x^i \equiv 1 + x^p \pmod{p} $$

$$ [x^m] (1+x)^n = \binom{n}{m} $$

$$ n = n/p \times p + n \bmod p $$

$$ (1+x)^n = (1+x)^{n/p \times p + n \bmod p} = (1+x)^{n/p \times p} \times (1+x)^{n \bmod p} $$

$$ (1+x)^{n/p \times p} = ((1+x)^p)^{n/p} \equiv (1+x^p)^{n/p} = \sum\limits_{i \ge 0} \binom{n/p}{i} x^{pi} $$

$$ (1+x)^{n \bmod p } = \sum\limits_{i=0}^{n \bmod p} \binom{n \bmod p}{i} x^i, n \bmod p < p $$

$$ m = m/p \times p + m \bmod p $$

$$ [x^m] (1+x)^{n/p \times p} \times (1+x)^{n \bmod p} = [x^{m/p \times p}] (1+x)^{n/p \times p} \times [x^{m \bmod p}] (1 + x) ^{n \bmod p} $$

$$ \binom{n/p}{m/p} \times \binom{n \bmod p}{m \bmod p} $$

---

$$ \binom{n}{m} \equiv \binom{n \bmod 2}{m \bmod 2} \binom{n/2}{m/2} \equiv \binom{n \bmod 2}{m \bmod 2} \binom{n/2 \bmod 2}{m/2 \bmod 2} \binom{n/4}{m/4} \equiv .... $$

$$ n = \overline{a_0 a_1 a_2 a_3 a_4 a_5 ...}_2 = \sum\limits_{i \ge 0} a_i 2^i $$

$$ m = \sum\limits_{i \ge 0} b_i 2^i $$

$$ \binom{n}{m} \equiv \binom{a_0}{b_0} \times \binom{a_1}{b_1} \times \binom{a_2}{b_2} \times \binom{a_3}{b_3} ... $$

$$ \forall i, a_i \ge b_i $$

$$ n = 10011100110010 $$

$$ m = 10000100100010 $$

$$ a_k \to b_{i,j} = \binom{i}{k-j} $$

$$ b_{i,j} = \prod a_k^{\binom{i}{k-j}} $$  
$$ E(X^4)=\frac{1}{\binom{n+1}{2}}(\sum\limits_{d=1}^{n}d^4 (n+1-d)+2\sum\limits_{d=1}^{n}d^2(n+1-2d)\sum\limits_{d\prime=1}^{n}d\prime^2 $$
$$ E(X^2)=\sum\limits_{d=1}^{n}d^2(n+1-d) = (n+1) \frac{n(n+1)(2n+1)}{6} - \frac{n^2(n+1)^2}{4} $$
$$ \frac{(n+1)(2n+1)}{6} - \frac{n(n+1)}{4} $$
$$ E(X^2)=\sum_{i=1}^{n}\sum_{j=i+1}^{n+1}(j-i)^2 \times \frac{1}{\binom{n+1}{2}} $$
$$ \frac{(n+1)n}{2} $$
$$ E(X^4)= $$
$$ E(X^2)=E(\sum_{i=1}^{n(n+1)/2}a_i^2+2\sum_{1\le i < j \le n(n+1)/2}a_ia_j) $$
$$ E(X^2)=\frac{n(n+1)}{2} $$
$$ a_i=a_j=a_k=a_l $$
-1 -1 -1 -1 
1 1 1 1
$$ E(X^4)=E(X^2)^2 + \binom{n+1}{2} \times \binom{n-1}{2} \times 2^{n-2};  $$


 我有2个岗位
 现在有10个候选人
 $$ \binom{2}{10}=\frac{2!}{(10-2)!2!} $$