$$ \phi(n)=n\prod\limits_{p\in P}\ 1-\frac{1}{p} $$
$$ \phi(n)\prod\limits_{p\in P} p=n\prod\limits_{p\in P}p-1 $$
$$ =\prod(p_i-1)p_i^{c_i-1} $$
$$ \sum\limits_{i=l}^r \text{qiandao(i)}\mod 666623333 $$
$$ =\sum\limits_{i=l}^r i-\phi(i)\mod 666623333$$

$$ \sum\limits_{i=l}^ri-\sum\limits_{i=l}^r\phi(i) \mod  666623333 $$
$$ \sum\limits_{i=l}^ri-\sum\limits_{i=l}^r\prod(p_i-1)p_i^{c_i-1} $$
$$ \sum\limits_{i=l}^ri-p_i^{c_i-1}\sum\limits_{i=l}^r\prod(p_i-1) $$
$$ \sum\limits_{i=l}^ri-p_i^{c_i-1}\sum\limits_{i=l}^r\prod p_i-\sum\limits_{i=l}^ri $$
$$ -p_i^{c_i-1}\sum\limits_{i=l}^r\prod p_i $$
$$ \sum\limits_{i=l}^r\prod p_i-p_i^{c_i-1} $$
---
$$ \phi(n)\prod\limits_{p\in P} p=n\prod\limits_{p\in P}p-1 $$
$$ \phi(n)=\frac{n(\prod\limits_ {p\in P}p-\prod\limits_ {p\in P}1)}{\prod\limits_{p \in P}p} $$
$$ \phi(n)=\frac{n\prod\limits_ {p\in P}p-n\prod\limits_ {p\in P}1}{\prod\limits_{p \in P}p} $$
$$ \phi(n)=(n-1)\prod\limits_ {p\in P}p-n\prod\limits_ {p\in P}1 $$

